Change REPL constructor semantics
Now when a module raises an exception, all of its constructors are added
to the operational semantics' constructor environment, not just the
constructors whose type definitions were reached.  There are type
soundness theorems for doing the update either way.

semantics/replScript.sml
@@ -66,12 +66,20 @@ val strip_mod_env_def = Define `
 strip_mod_env tenvM =
   MAP (\(n,tenv). (n,[])) tenvM`;
 
-val tenvC_to_envC_def = Define `
-tenvC_to_envC tenvC =
-  MAP (λ(cn,(tvs, ts, t)). (cn, (LENGTH ts, t))) tenvC`;
+val dec_to_cenv_def = Define `
+(dec_to_cenv mn (Dtype tds) = build_tdefs mn tds) ∧
+(dec_to_cenv mn _ = [])`;
+
+val decs_to_cenv_def = Define `
+(decs_to_cenv mn [] = []) ∧
+(decs_to_cenv mn (d::ds) = decs_to_cenv mn ds ++ dec_to_cenv mn d)`;
+
+val top_to_cenv_def = Define `
+(top_to_cenv (Tdec d) = dec_to_cenv NONE d) ∧
+(top_to_cenv (Tmod mn _ ds) = decs_to_cenv (SOME mn) ds)`;
 
 val update_repl_state_def = Define `
-update_repl_state state type_bindings ctors tenvM tenvC tenv store envC r =
+update_repl_state ast state type_bindings ctors tenvM tenvC tenv store envC r =
   case r of
     | Rval (envM,envE) =>
         <| type_bindings := type_bindings ++ state.type_bindings;
@@ -96,7 +104,7 @@ update_repl_state state type_bindings ctors tenvM tenvC tenv store envC r =
         * they don't go in the constructor type environment, the programmer
         * can't refer to any of them, so it doesn't matter much. *)
         state with <| store := store; 
-                      envC := envC ++ state.envC; 
+                      envC := top_to_cenv ast ++ state.envC; 
                       envM := strip_mod_env tenvM ++ state.envM;
                       tenvM := strip_mod_env tenvM ++ state.tenvM |>`;
 
@@ -144,7 +152,7 @@ val (ast_repl_rules, ast_repl_ind, ast_repl_cases) = Hol_reln `
    (type_bindings', ctors', top)) ∧
   (type_top state.tenvM state.tenvC state.tenv top tenvM' tenvC' tenv') ∧
   evaluate_top state.envM state.envC state.store state.envE top (store',envC',r) ∧
-  ast_repl (update_repl_state state type_bindings' ctors' tenvM' tenvC' tenv' store' envC' r) type_errors asts rest
+  ast_repl (update_repl_state top state type_bindings' ctors' tenvM' tenvC' tenv' store' envC' r) type_errors asts rest
   ⇒
   ast_repl state (F::type_errors) (SOME ast::asts) (Result (print_result top envC' r) rest)) ∧
 
